\documentclass{article}

% Formatting
\usepackage[utf8]{inputenc}
\usepackage[margin=1in]{geometry}
\usepackage[titletoc,title]{appendix}

% Math
\usepackage{amsmath,amsfonts,amssymb,mathtools}

% Algorithms
\usepackage[ruled,vlined]{algorithm2e}
\usepackage{algorithmic}

% Code syntax highlighting
\usepackage{minted}
\usemintedstyle{borland}

\title{Homework 1}
\author{David Trinh}
\date{September 17, 2024}

\begin{document}

\maketitle

\begin{itemize}
    \item\textbf{ Question 1}
        \begin{equation}
            r=\sum^{n-1}_{i=1} \sum^{n}_{j=i+1} \sum^{n}_{k=1} 1
        \end{equation}
        \begin{equation}
            r=\sum^{n-1}_{i=1} \sum^{n}_{j=i+1} n
        \end{equation}
        \begin{equation}
            r=n\sum^{n-1}_{i=1} (n-i)
        \end{equation}
        \begin{equation}
            r=n\left(\sum^{n-1}_{i=1} n - \sum^{n-1}_{i=1} i \right)
        \end{equation}
        \begin{equation}
            r=n^2\sum^{n-1}_{i=1} 1 - n\sum^{n-1}_{i=1} i
        \end{equation}
        \begin{equation}
            r=n^2(n-1) - n\left(\frac{n(n-1)}{2}\right)
        \end{equation}
        \begin{equation}
            r=n^2(n-1) - \frac{n^2(n-1)}{2}
        \end{equation}
        \begin{equation}
            r=\frac{n^2(n-1)}{2}
        \end{equation}
        \begin{equation}
            r=\frac{n^3-n^2}{2}
        \end{equation}
        \begin{itemize}
            \item[] Big-O: $O(n^3)$
            \item[] Big-$\Omega$: $\Omega(n^3)$
            \item[] Big-$\Theta$: $\Theta(n^3)$
        \end{itemize}

    \item\textbf{ Question 2}
        \begin{equation}
            r=\sum^{n}_{i=1} \sum^{i}_{j=1} \sum^{i+j}_{k=j} 1
        \end{equation}
        \begin{equation}
            r=\sum^{n}_{i=1} \sum^{i}_{j=1} (i+1)
        \end{equation}
        \begin{equation}
            r=\sum^{n}_{i=1} i(i+1)
        \end{equation}
        \begin{equation}
            r=\sum^{n}_{i=1} i^2 + \sum^{n}_{i=1} i
        \end{equation}
        \begin{equation}
            r=\frac{n(n+1)(2n+1)}{6} + \frac{n(n+1)}{2}
        \end{equation}
        \begin{equation}
            r=\frac{(n^2+n)(2n+1) + 3(n^2+n)}{6}
        \end{equation}
        \begin{equation}
            r=\frac{2n^3 + n^2 + 2n^2 + n + 3n^2 + 3n}{6}
        \end{equation}
        \begin{equation}
            r=\frac{n^3 + 3n^2 + 2n}{3}
        \end{equation}
        \begin{itemize}
            \item[] Big-O: $O(n^3)$
            \item[] Big-$\Omega$: $\Omega(n^3)$
            \item[] Big-$\Theta$: $\Theta(n^3)$
        \end{itemize}
\end{itemize}

\end{document}